lec7

ws/main.s
@@ -1,7 +1,6 @@
-
 section .text
 extern error
-global our_code_starts_here
+extern print
 
 error_non_number:
   push eax
@@ -9,36 +8,96 @@ error_non_number:
   call error
   add esp, 4 * 2
 
+
+error_non_bool:
+  push eax
+  push 2
+  call error
+  add esp, 4 * 2
+
+f:
+push ebp
+mov ebp, esp
+sub esp, 8
+mov eax, dword [ebp + 4 * 2]
+mov dword [ebp + 4 * -1], eax
+mov eax, dword [ebp + 4 * 3]
+mov dword [ebp + 4 * -2], eax
+mov eax, dword [ebp + 4 * -2]
+test eax, 1
+jnz error_non_number
+mov eax, dword [ebp + 4 * -1]
+test eax, 1
+jnz error_non_number
+add eax, dword [ebp + 4 * -2]
+mov dword [ebp + 4 * -1], eax
+mov eax, dword [ebp + 4 * 4]
+mov dword [ebp + 4 * -2], eax
+mov eax, dword [ebp + 4 * -2]
+test eax, 1
+jnz error_non_number
+mov eax, dword [ebp + 4 * -1]
+test eax, 1
+jnz error_non_number
+sub eax, dword [ebp + 4 * -2]
+mov esp, ebp
+pop ebp
+ret
+
+global our_code_starts_here
 our_code_starts_here:
+push ebp
+mov ebp, esp
+sub esp, 16
 mov eax, 2
 test eax, 1
 jnz error_non_number
-mov dword [esp + 4 * -1], eax
-mov eax, dword [esp + 4 * -1]
+mov dword [ebp + 4 * -1], eax
+mov eax, 6
 test eax, 1
 jnz error_non_number
-mov eax, 0
-sub eax, dword [esp + 4 * -1]
-mov dword [esp + 4 * -1], eax
+mov dword [ebp + 4 * -2], eax
 mov eax, 4
 test eax, 1
 jnz error_non_number
-mov dword [esp + 4 * -2], eax
-mov eax, dword [esp + 4 * -2]
+mov dword [ebp + 4 * -3], eax
+mov eax, dword [ebp + 4 * -3]
+push eax
+mov eax, dword [ebp + 4 * -2]
+push eax
+mov eax, dword [ebp + 4 * -1]
+push eax
+call f
+add esp, 12
+mov dword [ebp + 4 * -1], eax
+mov eax, 6
 test eax, 1
 jnz error_non_number
-mov eax, 0
-sub eax, dword [esp + 4 * -2]
-mov dword [esp + 4 * -2], eax
-mov eax, dword [esp + 4 * -2]
+mov dword [ebp + 4 * -2], eax
+mov eax, 12
 test eax, 1
 jnz error_non_number
-mov eax, dword [esp + 4 * -1]
+mov dword [ebp + 4 * -3], eax
+mov eax, 4
 test eax, 1
 jnz error_non_number
-cmp eax, dword [esp + 4 * -2]
-mov eax, 2147483649
-jle label_less_eq_0
-mov eax, 1
-label_less_eq_0:
+mov dword [ebp + 4 * -4], eax
+mov eax, dword [ebp + 4 * -4]
+push eax
+mov eax, dword [ebp + 4 * -3]
+push eax
+mov eax, dword [ebp + 4 * -2]
+push eax
+call f
+add esp, 12
+mov dword [ebp + 4 * -2], eax
+mov eax, dword [ebp + 4 * -2]
+test eax, 1
+jnz error_non_number
+mov eax, dword [ebp + 4 * -1]
+test eax, 1
+jnz error_non_number
+add eax, dword [ebp + 4 * -2]
+mov esp, ebp
+pop ebp
 ret
